TotalViperState.thy
@@ -70,13 +70,13 @@ type_synonym 'a total_trace = "label \<rightharpoonup> 'a total_state"
 type_synonym 'a store = "var \<rightharpoonup> 'a val" (* De Bruijn indices *)
 type_synonym 'a full_total_state = "'a store \<times> 'a total_trace \<times> 'a total_state"
 
-subsection \<open>Destructors for (full) total state\<close>
+section \<open>Destructors for (full) total state\<close>
 
 (*lift_definition get_heap_total :: "'a total_state \<Rightarrow> 'a total_heap" is "snd" done*)
-(*fun get_m_total :: "'a total_state \<Rightarrow> mask \<times> 'a predicate_mask"
+(*fun get_m_total :: "'a total_stateotal_full  \<Rightarrow> mask \<times> 'a predicate_mask"
   where "get_m_total \<phi> = get_m_pre_total (Rep_total_state \<phi>)"*)
 
-text\<open>Heap destructors total state\<close>
+subsection \<open>Heap destructors total state\<close>
 
 fun get_h_total :: "'a total_state \<Rightarrow> 'a total_heap \<times> 'a predicate_heap" 
   where "get_h_total \<phi> = get_h_pre_total (Rep_total_state \<phi>)"
@@ -87,7 +87,13 @@ fun get_hh_total :: "'a total_state \<Rightarrow> 'a total_heap"
 fun get_hp_total :: "'a total_state \<Rightarrow> 'a predicate_heap" 
   where "get_hp_total \<phi> = get_hp_pre_total (Rep_total_state \<phi>)"
 
-text\<open>Mask destructors total state\<close>
+lemma get_hh_from_h_total: "get_hh_total \<phi> = fst (get_h_total \<phi>)"
+  by simp
+
+lemma get_hp_from_h_total: "get_hp_total \<phi> = snd (get_h_total \<phi>)"
+  by simp
+
+subsection \<open>Mask destructors total state\<close>
 
 fun get_m_total :: "'a total_state \<Rightarrow> mask \<times> 'a predicate_mask" 
   where "get_m_total \<phi> = get_m_pre_total (Rep_total_state \<phi>)"
@@ -101,7 +107,13 @@ fun get_mp_total :: "'a total_state \<Rightarrow> 'a predicate_mask"
 lemma get_mask_total_wf: "wf_mask_simple (get_mh_total \<phi>)"
   using Rep_total_state by auto
 
-text\<open>Top-level constructors full total state\<close>
+lemma get_mh_from_m_total: "get_mh_total \<phi> = fst (get_m_total \<phi>)"
+  by simp
+
+lemma get_mp_from_m_total: "get_mp_total \<phi> = snd (get_m_total \<phi>)"
+  by simp
+
+subsection \<open>Top-level constructors full total state\<close>
 
 fun get_store_total :: "'a full_total_state \<Rightarrow> 'a store" 
   where "get_store_total \<omega> = fst \<omega>"
@@ -112,7 +124,7 @@ fun get_trace_total :: "'a full_total_state \<Rightarrow> 'a total_trace"
 fun get_total_full :: "'a full_total_state \<Rightarrow> 'a total_state"
   where "get_total_full \<omega> = snd (snd \<omega>)"
 
-text\<open>Heap destructors full total state\<close>
+subsection \<open>Heap destructors full total state\<close>
 
 fun get_h_total_full :: "'a full_total_state \<Rightarrow> 'a total_heap \<times> 'a predicate_heap"
   where "get_h_total_full \<omega> = get_h_total (get_total_full \<omega>)"
@@ -121,48 +133,76 @@ fun get_hh_total_full :: "'a full_total_state \<Rightarrow> 'a total_heap"
   where "get_hh_total_full \<omega> = get_hh_total (get_total_full \<omega>)"
 
 fun get_hp_total_full :: "'a full_total_state \<Rightarrow> 'a predicate_heap" 
-  where "get_hp_total_full \<omega> = get_hp_total (get_total_full \<omega>)"                   
+  where "get_hp_total_full \<omega> = get_hp_total (get_total_full \<omega>)"
 
-text\<open>Mask destructors full total state\<close>
+lemma get_hh_from_h_total_full: "get_hh_total_full \<phi> = fst (get_h_total_full \<phi>)"
+  by simp
+
+lemma get_hp_from_h_total_full: "get_hp_total_full \<phi> = snd (get_h_total_full \<phi>)"
+  by simp
+
+subsection \<open>Mask destructors full total state\<close>
 
 fun get_m_total_full :: "'a full_total_state \<Rightarrow> mask \<times> 'a predicate_mask"
   where "get_m_total_full \<omega> = get_m_total (get_total_full \<omega>)"
 
 fun get_mh_total_full :: "'a full_total_state \<Rightarrow> mask" where "get_mh_total_full \<omega> = get_mh_total (get_total_full \<omega>)"
 
-fun get_mp_total_full :: "'a full_total_state \<Rightarrow> 'a predicate_mask" where "get_mp_total_full \<omega> = get_mp_total (get_total_full \<omega>)"                   
+fun get_mp_total_full :: "'a full_total_state \<Rightarrow> 'a predicate_mask" where "get_mp_total_full \<omega> = get_mp_total (get_total_full \<omega>)"
 
-(*
+lemma get_mh_from_m_total_full: "get_mh_total_full \<phi> = fst (get_m_total_full \<phi>)"
+  by simp
+
+lemma get_mp_from_m_total_full: "get_mp_total_full \<phi> = snd (get_m_total_full \<phi>)"
+  by simp
+
+section \<open>Lemmas for proving equality of states\<close>
+
+lemma total_mask_eq:
+  assumes "get_mh_total \<phi> = get_mh_total \<phi>'" and
+          "get_mp_total \<phi> = get_mp_total \<phi>'" 
+  shows "get_m_total \<phi> = get_m_total \<phi>'"
+  using assms
+  by (metis get_m_total.simps get_mh_pre_total.simps get_mh_total.simps get_mp_pre_total.simps get_mp_total.simps surjective_pairing)
+
+lemma total_heap_eq:
+  assumes "get_hh_total \<phi> = get_hh_total \<phi>'" and
+          "get_hp_total \<phi> = get_hp_total \<phi>'" 
+  shows "get_h_total \<phi> = get_h_total \<phi>'"
+  using assms
+  by (metis get_h_total.elims get_hh_pre_total.simps get_hh_total.elims get_hp_pre_total.simps get_hp_total.elims prod_eqI)
+
 lemma total_state_eq:
-  assumes "get_mask_total \<phi> = get_mask_total \<phi>'" and
-          "get_heap_total \<phi> = get_heap_total \<phi>'"
+  assumes "get_m_total \<phi> = get_m_total \<phi>'" and
+          "get_h_total \<phi> = get_h_total \<phi>'"
   shows "\<phi> = \<phi>'"
   using assms
-  by (metis Rep_total_state_inverse get_heap_total.simps get_mask_total.simps surjective_pairing)
-*)
+  by (metis Rep_total_state_inverse get_h_pre_total.simps get_h_total.simps get_m_pre_total.simps get_m_total.simps prod_eqI)
 
-(*
 lemma full_total_state_eq: 
   assumes "get_store_total \<omega> = get_store_total \<omega>'" and
           "get_trace_total \<omega> = get_trace_total \<omega>'" and 
-          "get_heap_total_full \<omega> = get_heap_total_full \<omega>'" and
-          "get_mask_total_full \<omega> = get_mask_total_full \<omega>'"
+          "get_total_full \<omega> = get_total_full \<omega>'"
         shows "\<omega> = \<omega>'"
-  using assms
-  by (metis Rep_total_state_inject get_heap_total.elims get_heap_total_full.elims get_total_full.elims get_mask_total.elims get_mask_total_full.elims get_store_total.elims get_trace_total.elims prod.expand) 
+  using assms 
+  by (metis get_store_total.simps get_total_full.simps get_trace_total.simps prod.exhaust_sel)
+  
+lemma full_total_state_eq_2: 
+  assumes "get_store_total \<omega> = get_store_total \<omega>'" and
+          "get_trace_total \<omega> = get_trace_total \<omega>'" and 
+          "get_m_total_full \<omega> = get_m_total_full \<omega>'" and
+          "get_h_total_full \<omega> = get_h_total_full \<omega>'"
+        shows "\<omega> = \<omega>'"
+  using assms full_total_state_eq
+  by (metis get_h_total_full.elims get_m_total_full.elims total_state_eq)
 
-
-lemma get_total_full_comp: "Rep_total_state (get_total_full \<omega>) = (get_mask_total_full \<omega>, get_heap_total_full \<omega>)"
+lemma get_mask_total_full_wf: "wf_mask_simple (get_mh_total_full \<omega>)"
+  using get_mask_total_wf
   by simp
 
-lemma get_mask_total_full_wf: "wf_mask_simple (get_mask_total_full \<omega>)"
-  using get_mask_total_wf
-  by (metis get_mask_total_full.elims)
-*)
-
+(*
 subsection \<open>Addition of total states\<close>
 
-(*
 fun compatible_pre_states_total :: "'a pre_total_state \<Rightarrow> 'a pre_total_state \<Rightarrow> bool"
   where
     "compatible_pre_states_total s1 s2 =    
@@ -174,9 +214,10 @@ fun compatible_pre_states_total :: "'a pre_total_state \<Rightarrow> 'a pre_tota
 definition add_total_heaps :: "'a total_heap \<Rightarrow> 'a total_heap \<Rightarrow> mask \<Rightarrow> 'a total_heap"
   where "add_total_heaps h1 h2 m2 = (\<lambda>l. if ((pgt (m2 l) pnone)) then h2 l else h1 l)"
 *)
-
+(*
 text \<open>For compatible states, always the heap value of the first state is taken if the second state 
 does not have positive permission to the corresponding location.\<close>
+?*)
 
 (*
 fun pre_plus_total :: "'a pre_total_state \<Rightarrow> 'a pre_total_state \<Rightarrow> 'a pre_total_state option" where
